## Task 2.3: Analyze Drift Contribution

We focus on the drift contribution to $\frac{d}{dt}\mathcal{V}(\rho_t)$, which is given by the first expectation term in the result of Task 2.2:
$$
\text{Drift Contribution} = \mathbb{E}\left[ \left\langle X_t - X^*, +\lambda P_{X_t}(X_{\alpha,t}) - \frac{\sigma^2 C_{n,k}'}{2} \|X_t - X_{\alpha,t}\|_F^2 X_t \right\rangle_F \right]
$$
where $C_{n,k}' = n - \frac{k+1}{2}$.

We can split this into two parts:

* **Part A:** The main drift component involving $\lambda$:
    $$\text{Part A} = \mathbb{E}\left[ \left\langle X_t - X^*, +\lambda P_{X_t}(X_{\alpha,t}) \right\rangle_F \right]$$
* **Part B:** The contribution from the geometric correction term (part of the drift in the SDE):
    $$\text{Part B} = \mathbb{E}\left[ \left\langle X_t - X^*, - \frac{\sigma^2 C_{n,k}'}{2} \|X_t - X_{\alpha,t}\|_F^2 X_t \right\rangle_F \right]$$

Our goal is to analyze and bound each part. We begin with Part A.

### Analysis of Part A (Main Drift Component)

We analyze $\text{Part A} = \lambda \mathbb{E}\left[ \langle X_t - X^*, P_{X_t}(X_{\alpha,t}) \rangle_F \right]$.

1.  **Using $P_X(Y) = P_X(Y-X)$ and Self-Adjointness:**
    $$
    \text{Part A} = \lambda \mathbb{E}\left[ \langle X_t - X^*, P_{X_t}(X_{\alpha,t} - X_t) \rangle_F \right] \\
    = \lambda \mathbb{E}\left[ \langle P_{X_t}(X_t - X^*), X_{\alpha,t} - X_t \rangle_F \right]
    $$
2.  **Adding and Subtracting $X^*$:**
    $$
    = \lambda \mathbb{E}\left[ \langle P_{X_t}(X_t - X^*), (X_{\alpha,t} - X^*) - (X_t - X^*) \rangle_F \right] \\
    = \underbrace{\lambda \mathbb{E}\left[ \langle P_{X_t}(X_t - X^*), X_{\alpha,t} - X^* \rangle_F \right]}_{\text{Part A.1}} \underbrace{- \lambda \mathbb{E}\left[ \langle P_{X_t}(X_t - X^*), X_t - X^* \rangle_F \right]}_{\text{Part A.2}}
    $$
3.  **Analysis of Part A.2:** Using $\langle P_Y Z, Z \rangle_F = \|P_Y Z\|_F^2$ and the orthogonal decomposition $\|Y\|_F^2 = \|P_X Y\|_F^2 + \|N_X Y\|_F^2$:
    $$
    \text{Part A.2} = - \lambda \mathbb{E}\left[ \|P_{X_t}(X_t - X^*)\|_F^2 \right] \\
    = - \lambda \mathbb{E}\left[ \|X_t - X^*\|_F^2 - \|N_{X_t}(X_t - X^*)\|_F^2 \right] \\
    = - 2\lambda \mathcal{V}(\rho_t) + \lambda \mathbb{E}\left[ \|N_{X_t}(X_t - X^*)\|_F^2 \right]
    $$
4.  **Analysis of Part A.1:** Using Cauchy-Schwarz, $\|P_X Y\| \le \|Y\|$, and Young's inequality ($ab \le \frac{\delta}{2}a^2 + \frac{1}{2\delta}b^2$) for any $\delta > 0$:
    $$
    \text{Part A.1} \le \lambda \mathbb{E}\left[ \|P_{X_t}(X_t - X^*)\|_F \|X_{\alpha,t} - X^*\|_F \right] \\
    \le \lambda \mathbb{E}\left[ \|X_t - X^*\|_F \|X_{\alpha,t} - X^*\|_F \right] \\
    \le \lambda \mathbb{E}\left[ \frac{\delta}{2} \|X_t - X^*\|_F^2 + \frac{1}{2\delta} \|X_{\alpha,t} - X^*\|_F^2 \right] \\
    = \lambda \delta \mathcal{V}(\rho_t) + \frac{\lambda}{2\delta} \mathbb{E}[\|X_{\alpha,t} - X^*\|_F^2]
    $$
5.  **Combined Bound for Part A:** Summing the results for Part A.1 and Part A.2:
    $$
    \text{Part A} = \text{Part A.1} + \text{Part A.2} \\
    \le \left( -2\lambda + \lambda \delta \right) \mathcal{V}(\rho_t) + \lambda \mathbb{E}\left[ \|N_{X_t}(X_t - X^*)\|_F^2 \right] + \frac{\lambda}{2\delta} \mathbb{E}[\|X_{\alpha,t} - X^*\|_F^2]
    $$

---
### Analysis of Part B (Geometric Drift Component)

This task analyzes the contribution from the geometric correction component within the drift term to the evolution of $\mathcal{V}(\rho_t)$.

---

We now analyze:
    $$
    \text{Part B} = \mathbb{E}\left[ \left\langle X_t - X^*, - \frac{\sigma^2 C_{n,k}'}{2} \|X_t - X_{\alpha,t}\|_F^2 X_t \right\rangle_F \right]
    $$
    $$
    = -\frac{\sigma^2 C_{n,k}'}{2} \mathbb{E}\left[ \|X_t - X_{\alpha,t}\|_F^2 \langle X_t - X^*, X_t \rangle_F \right]
    $$
    where $C_{n,k}' = n - \frac{k+1}{2}$.

1.  **Analyze the Inner Product:**
    We analyze the inner product $\langle X_t - X^*, X_t \rangle_F$:
    $$
    \langle X_t - X^*, X_t \rangle_F = \text{Tr}((X_t - X^*)^T X_t) = \text{Tr}(X_t^T X_t) - \text{Tr}((X^*)^T X_t)
    $$
    Since $X_t \in V(n,k)$, $\text{Tr}(X_t^T X_t) = k$.
    $$
    \langle X_t - X^*, X_t \rangle_F = k - \text{Tr}((X^*)^T X_t)
    $$
    Relating this to the squared distance $\|X_t - X^*\|_F^2$:
    $$
    \|X_t - X^*\|_F^2 = \text{Tr}((X_t - X^*)^T (X_t - X^*)) \\
    = \text{Tr}(X_t^T X_t) - 2 \text{Tr}((X^*)^T X_t) + \text{Tr}((X^*)^T X^*)
    $$
    Since $X_t, X^* \in V(n,k)$, $\text{Tr}(X_t^T X_t) = k$ and $\text{Tr}((X^*)^T X^*) = k$.
    $$
    \|X_t - X^*\|_F^2 = k - 2 \text{Tr}((X^*)^T X_t) + k = 2(k - \text{Tr}((X^*)^T X_t))
    $$
    Therefore, the identity holds:
    $$
    \langle X_t - X^*, X_t \rangle_F = k - \text{Tr}((X^*)^T X_t) = \frac{1}{2} \|X_t - X^*\|_F^2
    $$

2.  **Substitute into Part B:**
    Substitute this identity back into the expression for Part B:
    $$
    \text{Part B} = -\frac{\sigma^2 C_{n,k}'}{2} \mathbb{E}\left[ \|X_t - X_{\alpha,t}\|_F^2 \left( \frac{1}{2} \|X_t - X^*\|_F^2 \right) \right]
    $$
    $$
    = -\frac{\sigma^2 C_{n,k}'}{4} \mathbb{E}\left[ \|X_t - X_{\alpha,t}\|_F^2 \|X_t - X^*\|_F^2 \right]
    $$

3.  **Conclusion for Part B:**
    Since $\|X_t - X_{\alpha,t}\|_F^2 \ge 0$, $\|X_t - X^*\|_F^2 \ge 0$, $\sigma^2 \ge 0$, and $C_{n,k}' = n - (k+1)/2 > 0$ (assuming $n > (k+1)/2$), the expectation is non-negative. Therefore:
    $$
    \boxed{
    \text{Part B} = -\frac{\sigma^2 C_{n,k}'}{4} \mathbb{E}\left[ \|X_t - X_{\alpha,t}\|_F^2 \|X_t - X^*\|_F^2 \right] \le 0
    }
    $$
    The contribution from the geometric correction term within the drift is always **non-positive**.

---