## Lemma 3: Differential Inequality for the Energy Functional on V(n,k)

**Lemma 3.** Let the following hold:

* $X_t$ follows the CBO SDE dynamics on $V(n,k)$ with law $\rho_t$.
* $\mathcal{V}(\rho_t) = \frac{1}{2}\mathbb{E}[\|X_t - X^*\|_F^2]$ is the energy functional, where $X^*$ is the global minimizer.
* $C_{n,k}' = n - (k+1)/2$.

Then, for any $\delta > 0$, the time evolution of $\mathcal{V}(\rho_t)$ satisfies:

$$
    \frac{d}{dt}\mathcal{V}(\rho_t) \le \left[ - \lambda (2 - C_N - \delta) + \left(\frac{\lambda}{2\delta} + \sigma^2 k C_{n,k}'\right) C_L + 2\sigma^2 k C_{n,k}' \right] \mathcal{V}(\rho_t) \\
    + \left[ \frac{\lambda}{2\delta} + \sigma^2 k C_{n,k}' \right] \epsilon_L(\alpha)
$$

---

### Proof

**1. Starting Point:** From Task 2.2, the evolution equation is:

$$
    \frac{d}{dt}\mathcal{V}(\rho_t) = \underbrace{\mathbb{E}\left[ \langle X_t - X^*, +\lambda P_{X_t}(X_{\alpha,t}) \rangle_F \right]}_{\text{Part A}} + \underbrace{\mathbb{E}\left[ \langle X_t - X^*, - \frac{\sigma^2 C_{n,k}'}{2} \|X_t - X_{\alpha,t}\|_F^2 X_t \rangle_F \right]}_{\text{Part B}} \\
    + \underbrace{\mathbb{E}\left[ \frac{\sigma^2 k C_{n,k}'}{2} \|X_t - X_{\alpha,t}\|_F^2 \right]}_{\text{Diffusion Term}}
$$

**2. Bound Part A:** From Task 2.3 analysis:

$$
    \text{Part A} \le \lambda \delta \mathcal{V}(\rho_t) + \frac{\lambda}{2\delta} \mathbb{E}[\|X_{\alpha,t} - X^*\|_F^2] - \lambda \mathbb{E}[\|P_{X_t}(X_t - X^*)\|_F^2]
$$

**3. Bound Part B:** From Task 2.3 analysis, Part B $\le 0$.

**4. Bound Diffusion Term:** From Task 2.4 analysis:
    
$$
    \text{Diffusion Term} \le 2\sigma^2 k C_{n,k}' \mathcal{V}(\rho_t) + \sigma^2 k C_{n,k}' \mathbb{E}[\|X_{\alpha,t} - X^*\|_F^2]
$$

**5. Combine Bounds:** Substitute the bounds for Part A, Part B ($\le 0$), and the Diffusion Term:

$$
    \frac{d}{dt}\mathcal{V}(\rho_t) \le \left[ \lambda \delta \mathcal{V}(\rho_t) + \frac{\lambda}{2\delta} \mathbb{E}[\|X_{\alpha,t} - X^*\|_F^2] - \lambda \mathbb{E}[\|P_{X_t}(X_t - X^*)\|_F^2] \right] \\
    + 0 \\
    + \left[ 2\sigma^2 k C_{n,k}' \mathcal{V}(\rho_t) + \sigma^2 k C_{n,k}' \mathbb{E}[\|X_{\alpha,t} - X^*\|_F^2] \right]
$$

**6. Use Lemma 1:** Relate the tangential component using $\mathbb{E}[\|P_{X_t}(X_t - X^*)\|_F^2] = 2\mathcal{V}(\rho_t) - \mathbb{E}[\|N_{X_t}(X_t - X^*)\|_F^2]$ and apply **Lemma 1**: $\mathbb{E}[\|N_{X_t}(X_t - X^*)\|_F^2] \le C_N \mathcal{V}(\rho_t)$. This gives:
    
$$-\lambda \mathbb{E}[\|P_{X_t}(X_t - X^*)\|_F^2] \le -\lambda (2 - C_N) \mathcal{V}(\rho_t)$$

**7. Substitute Tangential Bound:**
    
$$
    \frac{d}{dt}\mathcal{V}(\rho_t) \le \lambda \delta \mathcal{V}(\rho_t) + \frac{\lambda}{2\delta} \mathbb{E}[\|X_{\alpha,t} - X^*\|_F^2] - \lambda (2 - C_N) \mathcal{V}(\rho_t) \\
    + 2\sigma^2 k C_{n,k}' \mathcal{V}(\rho_t) + \sigma^2 k C_{n,k}' \mathbb{E}[\|X_{\alpha,t} - X^*\|_F^2]
$$

**8. Substitute Lemma 2:** Apply **Lemma 2**: $\mathbb{E}[\|X_{\alpha,t} - X^*\|_F^2] \le C_L \mathcal{V}(\rho_t) + \epsilon_L(\alpha)$:
    
$$
    \frac{d}{dt}\mathcal{V}(\rho_t) \le \lambda \delta \mathcal{V}(\rho_t) + \frac{\lambda}{2\delta} (C_L \mathcal{V}(\rho_t) + \epsilon_L(\alpha)) - \lambda (2 - C_N) \mathcal{V}(\rho_t) \\
    + 2\sigma^2 k C_{n,k}' \mathcal{V}(\rho_t) + \sigma^2 k C_{n,k}' (C_L \mathcal{V}(\rho_t) + \epsilon_L(\alpha))
$$

**9. Group Terms:** Collect terms multiplying $\mathcal{V}(\rho_t)$ and terms involving $\epsilon_L(\alpha)$:
    
$$
    \frac{d}{dt}\mathcal{V}(\rho_t) \le \left[ \lambda \delta + \frac{\lambda C_L}{2\delta} - \lambda (2 - C_N) + 2\sigma^2 k C_{n,k}' + \sigma^2 k C_{n,k}' C_L \right] \mathcal{V}(\rho_t) \\
    + \left[ \frac{\lambda}{2\delta} + \sigma^2 k C_{n,k}' \right] \epsilon_L(\alpha)
$$

Rearranging the coefficient of $\mathcal{V}(\rho_t)$:
    
$$
    \frac{d}{dt}\mathcal{V}(\rho_t) \le \left[ - \lambda (2 - C_N - \delta) + \frac{\lambda C_L}{2\delta} + 2\sigma^2 k C_{n,k}' (1 + \frac{C_L}{2}) \right] \mathcal{V}(\rho_t) \\
    + \left[ \frac{\lambda}{2\delta} + \sigma^2 k C_{n,k}' \right] \epsilon_L(\alpha)
$$

This yields the differential inequality stated in the lemma. $\square$