## Lemma 1: Bound on the Expected Squared Normal Component

**Lemma 1.** Let $X_t \in V(n,k)$ follow the CBO SDE dynamics, with $\rho_t = Law(X_t)$. Let $X^* \in V(n,k)$ be the global minimizer of $\mathcal{E}$. Let $P_X(Z) = Z - \frac{1}{2}(XZ^T X + XX^T Z)$ be the projection onto the tangent space $T_X V(n,k)$, and $N_X(Z) = (I - P_X)(Z)$ be the projection onto the normal space. Then, the expected squared Frobenius norm of the normal component of the error vector $(X_t - X^*)$ is bounded by twice the energy functional $\mathcal{V}(\rho_t) = \frac{1}{2}\mathbb{E}[\|X_t - X^*\|_F^2]$:
$$
\mathbb{E}\left[ \|N_{X_t}(X_t - X^*)\|_F^2 \right] \le 2 \mathcal{V}(\rho_t)
$$

---

### Proof

1.  **Formula for Normal Component:** The projection onto the normal space is given by $N_X(Z) = Z - P_X(Z)$. Using the formula for $P_X(Z)$ with $Z = X_t - X^*$, we found:
    $$N_{X_t}(X_t - X^*) = \frac{1}{2} \left( X_t(X_t - X^*)^T X_t + X_t X_t^T (X_t - X^*) \right)$$
    Let $S = X_t^T X^*$. This simplifies to:
    $$N_{X_t}(X_t - X^*) = X_t - \frac{1}{2} X_t ( S^T + S ) = X_t (I_k - \text{sym}(S))$$
    where $\text{sym}(S) = (S+S^T)/2$.

2.  **Calculate Squared Norm:** We calculate the squared Frobenius norm:
    $$\|N_{X_t}(X_t - X^*)\|_F^2 = \text{Tr}\left( (X_t (I_k - \text{sym}(S)))^T (X_t (I_k - \text{sym}(S))) \right)$$
    $$= \text{Tr}\left( (I_k - \text{sym}(S))^T X_t^T X_t (I_k - \text{sym}(S)) \right)$$
    Since $X_t^T X_t = I_k$:
    $$= \text{Tr}\left( (I_k - \text{sym}(S))^T (I_k - \text{sym}(S)) \right)$$
    Since $(I_k - \text{sym}(S))$ is symmetric:
    $$= \text{Tr}\left( (I_k - \text{sym}(S))^2 \right) = \|I_k - \text{sym}(S)\|_F^2$$
    Expanding the trace:
    $$= \text{Tr}(I_k - 2\text{sym}(S) + \text{sym}(S)^2) = k - 2\text{Tr}(\text{sym}(S)) + \text{Tr}(\text{sym}(S)^2)$$
    Since $\text{Tr}(\text{sym}(S)) = \text{Tr}(S)$:
    $$= k - 2\text{Tr}(S) + \text{Tr}(\text{sym}(S)^2)$$

3.  **Bound the $\text{Tr}(\text{sym}(S)^2)$ Term:** Let $A = \text{sym}(S)$. $A$ is a symmetric $k \times k$ matrix. The singular values $\sigma_j(S)$ of $S = X_t^T X^*$ satisfy $0 \le \sigma_j(S) \le 1$. The eigenvalues $\lambda_j(A)$ of $A$ satisfy $|\lambda_j(A)| \le \|A\|_{op} \le \|S\|_{op} \le 1$. Therefore:
    $$\text{Tr}(\text{sym}(S)^2) = \text{Tr}(A^2) = \sum_{j=1}^k (\lambda_j(A))^2 \le \sum_{j=1}^k 1^2 = k$$

4.  **Substitute Bound:** Substitute this bound back into the expression for the squared norm:
    $$\|N_{X_t}(X_t - X^*)\|_F^2 = k - 2\text{Tr}(S) + \text{Tr}(\text{sym}(S)^2) \le k - 2\text{Tr}(S) + k$$
    $$= 2k - 2\text{Tr}(S)$$

5.  **Relate to $\|X_t - X^*\|_F^2$:** Recall the identity $\|X_t - X^*\|_F^2 = 2k - 2 \text{Tr}(X_t^T X^*) = 2k - 2\text{Tr}(S)$.
    Substituting this gives:
    $$\|N_{X_t}(X_t - X^*)\|_F^2 \le \|X_t - X^*\|_F^2$$

6.  **Take Expectation:** Taking the expectation on both sides:
    $$\mathbb{E}[\|N_{X_t}(X_t - X^*)\|_F^2] \le \mathbb{E}[\|X_t - X^*\|_F^2]$$
    Using the definition $\mathcal{V}(\rho_t) = \frac{1}{2}\mathbb{E}[\|X_t - X^*\|_F^2]$, we have $\mathbb{E}[\|X_t - X^*\|_F^2] = 2\mathcal{V}(\rho_t)$.
    Therefore:
    $$\mathbb{E}[\|N_{X_t}(X_t - X^*)\|_F^2] \le 2\mathcal{V}(\rho_t)$$

This proves the lemma with $C_N = 2$.q